trying with no Phm

src/FcEtt/ett_ott.v
@@ -8,8 +8,7 @@ Definition index := nat. (*r indices *)
 
 Inductive role : Set :=  (*r Role *)
  | Nom : role
- | Rep : role
- | Phm : role.
+ | Rep : role.
 
 Inductive relflag : Set :=  (*r relevance flag *)
  | Rel : relflag
@@ -66,19 +65,19 @@ with co : Set :=  (*r explicit coercions *)
  | g_Left (g:co) (g':co)
  | g_Right (g:co) (g':co).
 
-Inductive sort : Set :=  (*r binding classifier *)
- | Tm (A:tm) (R:role)
- | Co (phi:constraint).
-
 Inductive sig_sort : Set :=  (*r signature classifier *)
  | Cs (A:tm) (R:role)
  | Ax (a:tm) (A:tm) (R:role).
 
-Definition context : Set := list ( atom * sort ).
+Inductive sort : Set :=  (*r binding classifier *)
+ | Tm (A:tm) (R:role)
+ | Co (phi:constraint).
 
 Definition available_props : Type := atoms.
 
 Definition sig : Set := list (atom * sig_sort).
+
+Definition context : Set := list ( atom * sort ).
 
 Definition role_context : Set := list ( atom * role ).
 
@@ -430,15 +429,6 @@ with lc_constraint : constraint -> Prop :=    (* defn lc_constraint *)
      (lc_tm A) ->
      (lc_constraint (Eq a b A R)).
 
-(* defns LC_sort *)
-Inductive lc_sort : sort -> Prop :=    (* defn lc_sort *)
- | lc_Tm : forall (A:tm) (R:role),
-     (lc_tm A) ->
-     (lc_sort (Tm A R))
- | lc_Co : forall (phi:constraint),
-     (lc_constraint phi) ->
-     (lc_sort (Co phi)).
-
 (* defns LC_sig_sort *)
 Inductive lc_sig_sort : sig_sort -> Prop :=    (* defn lc_sig_sort *)
  | lc_Cs : forall (A:tm) (R:role),
@@ -448,6 +438,15 @@ Inductive lc_sig_sort : sig_sort -> Prop :=    (* defn lc_sig_sort *)
      (lc_tm a) ->
      (lc_tm A) ->
      (lc_sig_sort (Ax a A R)).
+
+(* defns LC_sort *)
+Inductive lc_sort : sort -> Prop :=    (* defn lc_sort *)
+ | lc_Tm : forall (A:tm) (R:role),
+     (lc_tm A) ->
+     (lc_sort (Tm A R))
+ | lc_Co : forall (phi:constraint),
+     (lc_constraint phi) ->
+     (lc_sort (Co phi)).
 (** free variables *)
 Fixpoint fv_tm_tm_co (g_5:co) : vars :=
   match g_5 with
@@ -739,15 +738,11 @@ Definition min (r1 : role) (r2 : role) : role :=
   match r1 , r2 with
   | Nom, _   => Nom
   | _  , Nom => Nom
-  | Rep, _   => Rep
-  | _ , Rep  => Rep
-  | Phm, Phm => Phm
+  | Rep, Rep => Rep
   end.
 
 Definition max (r1 : role) (r2 : role) : role :=
   match r1 , r2 with
-  | _, Phm   => Phm
-  | Phm, _   => Phm
   | _, Rep   => Rep
   | Rep, _   => Rep
   | Nom, Nom => Nom
@@ -757,9 +752,7 @@ Definition lte_role (r1 : role) (r2 : role) : bool :=
   match r1 , r2 with
   | Nom, _   => true
   | Rep, Nom => false
-  | Rep, _   => true
-  | Phm, Phm => true
-  | _, _     => false
+  | Rep, Rep => true
   end.
 
 Fixpoint erase_tm (a : tm) (r : role) : tm :=
@@ -848,8 +841,8 @@ Fixpoint ctx_to_rctx (G : context) : role_context :=
 Inductive SubRole : role -> role -> Prop :=    (* defn SubRole *)
  | NomBot : forall (R:role),
      SubRole Nom R
- | PhmTop : forall (R:role),
-     SubRole R Phm
+ | RepTop : forall (R:role),
+     SubRole R Rep
  | Refl : forall (R:role),
      SubRole R R
  | Trans : forall (R1 R3 R2:role),
@@ -928,8 +921,10 @@ with Value : role -> tm -> Prop :=    (* defn Value *)
      Value R a ->
      Value R  ( (a_CApp a g_Triv) ) 
  | Value_Bullet : forall (R:role),
-     Value R a_Bullet
-with value_type : role -> tm -> Prop :=    (* defn value_type *)
+     Value R a_Bullet.
+
+(* defns JValueType *)
+Inductive value_type : role -> tm -> Prop :=    (* defn value_type *)
  | value_type_Star : forall (R:role),
      value_type R a_Star
  | value_type_Pi : forall (R:role) (rho:relflag) (A:tm) (R1:role) (B:tm),
@@ -999,12 +994,14 @@ Inductive erased_tm : role_context -> tm -> role -> Prop :=    (* defn erased_tm
  | erased_a_Pi : forall (L:vars) (W:role_context) (rho:relflag) (A:tm) (R1:role) (B:tm) (R:role),
      erased_tm W A R1 ->
       ( forall x , x \notin  L  -> erased_tm  (( x  ~  R1 ) ++  W )   ( open_tm_wrt_tm B (a_Var_f x) )  R )  ->
+     SubRole R1 R ->
      erased_tm W  ( (a_Pi rho A R1 B) )  R
  | erased_a_CPi : forall (L:vars) (W:role_context) (a b A:tm) (R1:role) (B:tm) (R:role),
      erased_tm W a R1 ->
      erased_tm W b R1 ->
      erased_tm W A R1 ->
       ( forall c , c \notin  L  -> erased_tm W  ( open_tm_wrt_co B (g_Var_f c) )  R )  ->
+     SubRole R1 R ->
      erased_tm W  ( (a_CPi (Eq a b A R1) B) )  R
  | erased_a_CAbs : forall (L:vars) (W:role_context) (b:tm) (R:role),
       ( forall c , c \notin  L  -> erased_tm W  ( open_tm_wrt_co b (g_Var_f c) )  R )  ->
@@ -1015,10 +1012,7 @@ Inductive erased_tm : role_context -> tm -> role -> Prop :=    (* defn erased_tm
  | erased_a_Fam : forall (W:role_context) (F:const) (R1:role) (a A:tm) (R:role),
       uniq  W  ->
       binds  F  ( (Ax a A R) )   toplevel   ->
-     erased_tm W (a_Fam F) R1
- | erased_a_Conv : forall (W:role_context) (a:tm) (R1 R:role),
-     erased_tm W a R ->
-     erased_tm W  ( (a_Conv a R1 g_Triv) )  R.
+     erased_tm W (a_Fam F) R1.
 
 (* defns JChk *)
 Inductive RhoCheck : relflag -> tmvar -> tm -> Prop :=    (* defn RhoCheck *)
@@ -1052,7 +1046,7 @@ Inductive Par : role_context -> tm -> tm -> role -> Prop :=    (* defn Par *)
       ( forall x , x \notin  L  -> Par  (( x  ~  R1 ) ++  W )   ( open_tm_wrt_tm a (a_Var_f x) )   ( open_tm_wrt_tm a' (a_Var_f x) )  R )  ->
      Par W (a_UAbs rho R1 a) (a_UAbs rho R1 a') R
  | Par_Pi : forall (L:vars) (W:role_context) (rho:relflag) (A:tm) (R1:role) (B A' B':tm) (R:role),
-     Par W A A' R1 ->
+     Par W A A' R ->
       ( forall x , x \notin  L  -> Par  (( x  ~  R1 ) ++  W )   ( open_tm_wrt_tm B (a_Var_f x) )   ( open_tm_wrt_tm B' (a_Var_f x) )  R )  ->
      Par W (a_Pi rho A R1 B) (a_Pi rho A' R1 B') R
  | Par_CAbs : forall (L:vars) (W:role_context) (a a':tm) (R:role),
@@ -1062,33 +1056,13 @@ Inductive Par : role_context -> tm -> tm -> role -> Prop :=    (* defn Par *)
      Par W A A' R1 ->
      Par W a a' R1 ->
      Par W b b' R1 ->
-      ( forall c , c \notin  L  -> Par W  ( open_tm_wrt_co B (g_Var_f c) )   ( open_tm_wrt_co B' (g_Var_f c) )  R )  ->
+      ( forall c , c \notin  L  -> Par W  ( open_tm_wrt_co B (g_Var_f c) )   ( open_tm_wrt_co B' (g_Var_f c) )  R1 )  ->
      Par W (a_CPi (Eq a b A R1) B) (a_CPi (Eq a' b' A' R1) B') R
  | Par_Axiom : forall (W:role_context) (F:const) (a:tm) (R:role) (A:tm) (R1:role),
       binds  F  ( (Ax a A R1) )   toplevel   ->
      SubRole R1 R ->
       uniq  W  ->
      Par W (a_Fam F) a R
- | Par_Cong : forall (W:role_context) (a1:tm) (R:role) (a2:tm) (R1:role),
-     Par W a1 a2 R1 ->
-     Par W (a_Conv a1 R g_Triv) (a_Conv a2 R g_Triv) R1
- | Par_Combine : forall (W:role_context) (a1:tm) (R:role) (a2:tm) (R1:role),
-     Par W a1  ( (a_Conv a2 R g_Triv) )  R1 ->
-     Par W  ( (a_Conv a1 R g_Triv) )   ( (a_Conv a2 R g_Triv) )  R1
- | Par_Push : forall (W:role_context) (a1:tm) (R2:role) (b1 a2 b2:tm) (R R1:role),
-     Par W a1  ( (a_Conv a2 R g_Triv) )  R1 ->
-     Par W b1 b2 R2 ->
-     Par W  (a_App  a1  Rel  R2   b1 )  (a_Conv  (  (a_App  a2  Rel  R2    ( (a_Conv b2 R g_Triv) )  )  )  R g_Triv) R1
- | Par_PushCombine : forall (W:role_context) (a1:tm) (R2:role) (b1 a2 b2:tm) (R R1:role),
-     Par W a1  ( (a_Conv a2 R g_Triv) )  R1 ->
-     Par W b1  ( (a_Conv b2 R g_Triv) )  R2 ->
-     Par W  (a_App  a1  Rel  R2   b1 )  (a_Conv  (  (a_App  a2  Rel  R2    ( (a_Conv b2 R g_Triv) )  )  )  R g_Triv) R1
- | Par_CPush : forall (W:role_context) (a1 a2:tm) (R R1:role),
-     Par W a1  ( (a_Conv a2 R g_Triv) )  R1 ->
-     Par W (a_CApp a1 g_Triv) (a_Conv  ( (a_CApp a2 g_Triv) )  R g_Triv) R1
- | Par_Bullet : forall (W:role_context) (a:tm),
-     erased_tm W a Phm ->
-     Par W a a_Bullet Phm
 with MultiPar : role_context -> tm -> tm -> role -> Prop :=    (* defn MultiPar *)
  | MP_Refl : forall (W:role_context) (a:tm) (R:role),
      lc_tm a ->
@@ -1116,9 +1090,6 @@ Inductive Beta : tm -> tm -> role -> Prop :=    (* defn Beta *)
       binds  F  ( (Ax a A R) )   toplevel   ->
      SubRole R R1 ->
      Beta (a_Fam F) a R1
- | Beta_Bullet : forall (a:tm),
-     lc_tm a ->
-     Beta a a_Bullet Phm
 with reduction_in_one : tm -> tm -> role -> Prop :=    (* defn reduction_in_one *)
  | E_AbsTerm : forall (L:vars) (R:role) (a a':tm) (R1:role),
       ( forall x , x \notin  L  -> reduction_in_one  ( open_tm_wrt_tm a (a_Var_f x) )   ( open_tm_wrt_tm a' (a_Var_f x) )  R1 )  ->
@@ -1141,20 +1112,6 @@ with reduction_in_one : tm -> tm -> role -> Prop :=    (* defn reduction_in_one 
       binds  F  ( (Ax a A R) )   toplevel   ->
      SubRole R R1 ->
      reduction_in_one (a_Fam F) a R1
- | E_Cong : forall (a:tm) (R:role) (a':tm) (R1:role),
-     reduction_in_one a a' R1 ->
-     reduction_in_one (a_Conv a R g_Triv) (a_Conv a' R g_Triv) R1
- | E_Combine : forall (v:tm) (R1 R2 R:role),
-     CoercedValue R  ( (a_Conv v R1 g_Triv) )  ->
-     SubRole R1 R2 ->
-     reduction_in_one (a_Conv  ( (a_Conv v R1 g_Triv) )  R2 g_Triv) (a_Conv v R2 g_Triv) R
- | E_Push : forall (v1:tm) (R:role) (rho:relflag) (R1:role) (b:tm) (R2:role),
-     lc_tm b ->
-     CoercedValue R2  ( (a_Conv v1 R g_Triv) )  ->
-     reduction_in_one (a_App  ( (a_Conv v1 R g_Triv) )  rho R1 b) (a_Conv  ( (a_App v1 rho R1  ( (a_Conv b R g_Triv) ) ) )  R g_Triv) R2
- | E_CPush : forall (v1:tm) (R R1:role),
-     CoercedValue R1  ( (a_Conv v1 R g_Triv) )  ->
-     reduction_in_one (a_CApp  ( (a_Conv v1 R g_Triv) )  g_Triv) (a_Conv  ( (a_CApp v1 g_Triv) )  R g_Triv) R1
 with reduction : tm -> tm -> role -> Prop :=    (* defn reduction *)
  | Equal : forall (a:tm) (R:role),
      lc_tm a ->
@@ -1165,12 +1122,13 @@ with reduction : tm -> tm -> role -> Prop :=    (* defn reduction *)
      reduction a a' R.
 
 (* defns Jett *)
-Inductive PropWff : context -> constraint -> Prop :=    (* defn PropWff *)
- | E_Wff : forall (G:context) (a b A:tm) (R:role),
-     Typing G a A R ->
-     Typing G b A R ->
-      ( Typing G A a_Star R )  ->
-     PropWff G (Eq a b A R)
+Inductive PropWff : context -> constraint -> role -> Prop :=    (* defn PropWff *)
+ | E_Wff : forall (G:context) (a b A:tm) (R1 R:role),
+     Typing G a A R1 ->
+     Typing G b A R1 ->
+      ( Typing G A a_Star R1 )  ->
+     SubRole R1 R ->
+     PropWff G (Eq a b A R1) R
 with Typing : context -> tm -> tm -> role -> Prop :=    (* defn Typing *)
  | E_SubRole : forall (G:context) (a A:tm) (R2 R1:role),
      SubRole R1 R2 ->
@@ -1186,11 +1144,13 @@ with Typing : context -> tm -> tm -> role -> Prop :=    (* defn Typing *)
  | E_Pi : forall (L:vars) (G:context) (rho:relflag) (A:tm) (R:role) (B:tm) (R':role),
       ( forall x , x \notin  L  -> Typing  (( x ~ Tm  A R ) ++  G )   ( open_tm_wrt_tm B (a_Var_f x) )  a_Star R' )  ->
       ( Typing G A a_Star R )  ->
+     SubRole R R' ->
      Typing G (a_Pi rho A R B) a_Star R'
  | E_Abs : forall (L:vars) (G:context) (rho:relflag) (R:role) (a A B:tm) (R':role),
       ( forall x , x \notin  L  -> Typing  (( x ~ Tm  A R ) ++  G )   ( open_tm_wrt_tm a (a_Var_f x) )   ( open_tm_wrt_tm B (a_Var_f x) )  R' )  ->
       ( Typing G A a_Star R )  ->
       ( forall x , x \notin  L  -> RhoCheck rho x  ( open_tm_wrt_tm a (a_Var_f x) )  )  ->
+     SubRole R R' ->
      Typing G (a_UAbs rho R a)  ( (a_Pi rho A R B) )  R'
  | E_App : forall (G:context) (b:tm) (R:role) (a B:tm) (R':role) (A:tm),
      Typing G b (a_Pi Rel A R B) R' ->
@@ -1202,16 +1162,16 @@ with Typing : context -> tm -> tm -> role -> Prop :=    (* defn Typing *)
      Typing G (a_App b Irrel R a_Bullet)  (open_tm_wrt_tm  B   a )  R'
  | E_Conv : forall (G:context) (a B:tm) (R:role) (A:tm),
      Typing G a A R ->
-     DefEq G  (dom  G )  A B a_Star R ->
+     DefEq G  (dom  G )  A B a_Star Rep ->
       ( Typing G B a_Star R )  ->
      Typing G a B R
  | E_CPi : forall (L:vars) (G:context) (phi:constraint) (B:tm) (R:role),
       ( forall c , c \notin  L  -> Typing  (( c ~ Co  phi ) ++  G )   ( open_tm_wrt_co B (g_Var_f c) )  a_Star R )  ->
-      ( PropWff G phi )  ->
+      ( PropWff G phi R )  ->
      Typing G (a_CPi phi B) a_Star R
  | E_CAbs : forall (L:vars) (G:context) (a:tm) (phi:constraint) (B:tm) (R:role),
       ( forall c , c \notin  L  -> Typing  (( c ~ Co  phi ) ++  G )   ( open_tm_wrt_co a (g_Var_f c) )   ( open_tm_wrt_co B (g_Var_f c) )  R )  ->
-      ( PropWff G phi )  ->
+      ( PropWff G phi R )  ->
      Typing G (a_UCAbs a) (a_CPi phi B) R
  | E_CApp : forall (G:context) (a1 B1:tm) (R':role) (a b A:tm) (R:role),
      Typing G a1 (a_CPi  ( (Eq a b A R) )  B1) R' ->
@@ -1220,29 +1180,21 @@ with Typing : context -> tm -> tm -> role -> Prop :=    (* defn Typing *)
  | E_Fam : forall (G:context) (F:const) (A:tm) (R1:role) (a:tm) (R:role),
      Ctx G ->
       binds  F  ( (Ax a A R) )   toplevel   ->
-     Typing  nil  A a_Star R1 ->
+     Typing  nil  A a_Star R ->
      Typing G (a_Fam F) A R1
- | E_TyCast : forall (G:context) (a:tm) (R2:role) (A2:tm) (R1:role) (A1:tm),
-     Typing G a A1 R1 ->
-     DefEq G  (dom  G )  A1 A2 a_Star R2 ->
-      ( Typing G A2 a_Star R1 )  ->
-     Typing G (a_Conv a R2 g_Triv) A2 R1
- | E_Bullet : forall (G:context) (A:tm),
-     Typing G A a_Star Phm ->
-     Typing G a_Bullet A Phm
-with Iso : context -> available_props -> constraint -> constraint -> Prop :=    (* defn Iso *)
- | E_PropCong : forall (G:context) (D:available_props) (A1 B1 A:tm) (R:role) (A2 B2:tm),
+with Iso : context -> available_props -> constraint -> constraint -> role -> Prop :=    (* defn Iso *)
+ | E_PropCong : forall (G:context) (D:available_props) (A1 B1 A:tm) (R1:role) (A2 B2:tm) (R:role),
      DefEq G D A1 A2 A R ->
      DefEq G D B1 B2 A R ->
-     Iso G D (Eq A1 B1 A R) (Eq A2 B2 A R)
- | E_IsoConv : forall (G:context) (D:available_props) (A1 A2 A:tm) (R:role) (B:tm),
+     Iso G D (Eq A1 B1 A R1) (Eq A2 B2 A R1) R
+ | E_IsoConv : forall (G:context) (D:available_props) (A1 A2 A:tm) (R1:role) (B:tm) (R:role),
      DefEq G D A B a_Star R ->
-     PropWff G (Eq A1 A2 A R) ->
-     PropWff G (Eq A1 A2 B R) ->
-     Iso G D (Eq A1 A2 A R) (Eq A1 A2 B R)
- | E_CPiFst : forall (G:context) (D:available_props) (a1 a2 A:tm) (R:role) (b1 b2 B B1 B2:tm) (R':role),
+     PropWff G (Eq A1 A2 A R1) R ->
+     PropWff G (Eq A1 A2 B R1) R ->
+     Iso G D (Eq A1 A2 A R1) (Eq A1 A2 B R1) R
+ | E_CPiFst : forall (G:context) (D:available_props) (a1 a2 A:tm) (R:role) (b1 b2 B:tm) (R':role) (B1 B2:tm),
      DefEq G D (a_CPi  ( (Eq a1 a2 A R) )  B1) (a_CPi  ( (Eq b1 b2 B R) )  B2) a_Star R' ->
-     Iso G D (Eq a1 a2 A R) (Eq b1 b2 B R)
+     Iso G D (Eq a1 a2 A R) (Eq b1 b2 B R) R'
 with DefEq : context -> available_props -> tm -> tm -> tm -> role -> Prop :=    (* defn DefEq *)
  | E_Assn : forall (G:context) (D:available_props) (a b A:tm) (R:role) (c:covar),
      Ctx G ->
@@ -1274,12 +1226,14 @@ with DefEq : context -> available_props -> tm -> tm -> tm -> role -> Prop :=    
       ( Typing G A1 a_Star R )  ->
       ( Typing G (a_Pi rho A1 R B1) a_Star R' )  ->
       ( Typing G (a_Pi rho A2 R B2) a_Star R' )  ->
+     SubRole R R' ->
      DefEq G D  ( (a_Pi rho A1 R B1) )   ( (a_Pi rho A2 R B2) )  a_Star R'
  | E_AbsCong : forall (L:vars) (G:context) (D:available_props) (rho:relflag) (R:role) (b1 b2 A1 B:tm) (R':role),
       ( forall x , x \notin  L  -> DefEq  (( x ~ Tm  A1 R ) ++  G )  D  ( open_tm_wrt_tm b1 (a_Var_f x) )   ( open_tm_wrt_tm b2 (a_Var_f x) )   ( open_tm_wrt_tm B (a_Var_f x) )  R' )  ->
       ( Typing G A1 a_Star R )  ->
       ( forall x , x \notin  L  -> RhoCheck rho x  ( open_tm_wrt_tm b1 (a_Var_f x) )  )  ->
       ( forall x , x \notin  L  -> RhoCheck rho x  ( open_tm_wrt_tm b2 (a_Var_f x) )  )  ->
+     SubRole R R' ->
      DefEq G D  ( (a_UAbs rho R b1) )   ( (a_UAbs rho R b2) )   ( (a_Pi rho A1 R B) )  R'
  | E_AppCong : forall (G:context) (D:available_props) (a1:tm) (R:role) (a2 b1 b2 B:tm) (R':role) (A:tm),
      DefEq G D a1 b1  ( (a_Pi Rel A R B) )  R' ->
@@ -1297,15 +1251,16 @@ with DefEq : context -> available_props -> tm -> tm -> tm -> role -> Prop :=    
      DefEq G D a1 a2 A1 R ->
      DefEq G D  (open_tm_wrt_tm  B1   a1 )   (open_tm_wrt_tm  B2   a2 )  a_Star R'
  | E_CPiCong : forall (L:vars) (G:context) (D:available_props) (a1 b1 A1:tm) (R:role) (A a2 b2 A2 B:tm) (R':role),
-     Iso G D (Eq a1 b1 A1 R) (Eq a2 b2 A2 R) ->
+     Iso G D (Eq a1 b1 A1 R) (Eq a2 b2 A2 R) R' ->
       ( forall c , c \notin  L  -> DefEq  (( c ~ Co  (Eq a1 b1 A1 R) ) ++  G )  D  ( open_tm_wrt_co A (g_Var_f c) )   ( open_tm_wrt_co B (g_Var_f c) )  a_Star R' )  ->
-      ( PropWff G (Eq a1 b1 A1 R) )  ->
+      ( PropWff G (Eq a1 b1 A1 R) R' )  ->
       ( Typing G (a_CPi (Eq a1 b1 A1 R) A) a_Star R' )  ->
       ( Typing G (a_CPi (Eq a2 b2 A2 R) B) a_Star R' )  ->
+     SubRole R R' ->
      DefEq G D (a_CPi (Eq a1 b1 A1 R) A) (a_CPi (Eq a2 b2 A2 R) B) a_Star R'
  | E_CAbsCong : forall (L:vars) (G:context) (D:available_props) (a b:tm) (phi1:constraint) (B:tm) (R:role),
       ( forall c , c \notin  L  -> DefEq  (( c ~ Co  phi1 ) ++  G )  D  ( open_tm_wrt_co a (g_Var_f c) )   ( open_tm_wrt_co b (g_Var_f c) )   ( open_tm_wrt_co B (g_Var_f c) )  R )  ->
-      ( PropWff G phi1 )  ->
+      ( PropWff G phi1 R )  ->
      DefEq G D  ( (a_UCAbs a) )   ( (a_UCAbs b) )  (a_CPi phi1 B) R
  | E_CAppCong : forall (G:context) (D:available_props) (a1 b1 B:tm) (R':role) (a b A:tm) (R:role),
      DefEq G D a1 b1  ( (a_CPi  ( (Eq a b A R) )  B) )  R' ->
@@ -1318,21 +1273,15 @@ with DefEq : context -> available_props -> tm -> tm -> tm -> role -> Prop :=    
      DefEq G D  (open_tm_wrt_co  B1   g_Triv )   (open_tm_wrt_co  B2   g_Triv )  a_Star R0
  | E_Cast : forall (G:context) (D:available_props) (a' b' A':tm) (R:role) (a b A:tm),
      DefEq G D a b A R ->
-     Iso G D (Eq a b A R) (Eq a' b' A' R) ->
+     Iso G D (Eq a b A R) (Eq a' b' A' R) Rep ->
      DefEq G D a' b' A' R
- | E_EqConv : forall (G:context) (D:available_props) (a b B:tm) (R2:role) (A:tm) (R1:role),
-     DefEq G D a b A R1 ->
-     DefEq G  (dom  G )  A B a_Star R2 ->
-      ( SubRole R1 R2 )  ->
-     DefEq G D a b B R2
- | E_IsoSnd : forall (G:context) (D:available_props) (A A':tm) (R:role) (a b a' b':tm),
-     Iso G D (Eq a b A R) (Eq a' b' A' R) ->
+ | E_EqConv : forall (G:context) (D:available_props) (a b B:tm) (R:role) (A:tm),
+     DefEq G D a b A R ->
+     DefEq G  (dom  G )  A B a_Star Rep ->
+     DefEq G D a b B R
+ | E_IsoSnd : forall (G:context) (D:available_props) (A A':tm) (R:role) (a b:tm) (R1:role) (a' b':tm),
+     Iso G D (Eq a b A R1) (Eq a' b' A' R1) R ->
      DefEq G D A A' a_Star R
- | E_CastCong : forall (G:context) (D:available_props) (a1:tm) (R2:role) (a2 B:tm) (R1:role) (A:tm),
-     DefEq G D a1 a2 A R1 ->
-     DefEq G  (dom  G )  A B a_Star R2 ->
-     Typing G B a_Star R1 ->
-     DefEq G D (a_Conv a1 R2 g_Triv) (a_Conv a2 R2 g_Triv) B R1
 with Ctx : context -> Prop :=    (* defn Ctx *)
  | E_Empty : 
      Ctx  nil 
@@ -1343,7 +1292,7 @@ with Ctx : context -> Prop :=    (* defn Ctx *)
      Ctx  (( x ~ Tm  A R ) ++  G ) 
  | E_ConsCo : forall (G:context) (c:covar) (phi:constraint),
      Ctx G ->
-     PropWff G phi ->
+     PropWff G phi Rep ->
       ~ AtomSetImpl.In  c  (dom  G )  ->
      Ctx  (( c ~ Co  phi ) ++  G ) .
 
@@ -1618,6 +1567,6 @@ Inductive head_reduction : context -> tm -> tm -> role -> Prop :=    (* defn hea
 
 
 (** infrastructure *)
-Hint Constructors SubRole Path CoercedValue Value value_type consistent erased_tm RhoCheck Par MultiPar joins Beta reduction_in_one reduction PropWff Typing Iso DefEq Ctx Sig AnnPropWff AnnTyping AnnIso AnnDefEq AnnCtx AnnSig head_reduction lc_co lc_brs lc_tm lc_constraint lc_sort lc_sig_sort.
+Hint Constructors SubRole Path CoercedValue Value value_type consistent erased_tm RhoCheck Par MultiPar joins Beta reduction_in_one reduction PropWff Typing Iso DefEq Ctx Sig AnnPropWff AnnTyping AnnIso AnnDefEq AnnCtx AnnSig head_reduction lc_co lc_brs lc_tm lc_constraint lc_sig_sort lc_sort.
 
 
