src/FcEtt/ett_par.v
@@ -30,15 +30,13 @@ Lemma par_app_rctx : forall W1 W2 W3 a a' R, uniq (W1 ++ W2 ++ W3) ->
                      Par (W1 ++ W2 ++ W3) a a' R.
 Proof. intros W1 W2 W3 a a' R U H. generalize dependent W2.
        dependent induction H; intros; eauto.
-        - econstructor. eapply erased_app_rctx; eauto.
+       all: try solve [econstructor; eauto 3 using erased_app_rctx].
         - eapply Par_Abs with (L := union L (dom (W1 ++ W2 ++ W3))).
           intros. rewrite <- app_assoc.
           eapply H0; eauto. simpl_env. auto.
         - eapply Par_Pi with (L := union L (dom (W1 ++ W2 ++ W3))); eauto.
           intros. rewrite <- app_assoc.
           eapply H1; eauto. simpl_env. auto.
-        - econstructor; eauto.
-        - econstructor. eapply erased_app_rctx; eauto.
 Qed.
 
 (* ------------------------------------------ *)
@@ -87,9 +85,10 @@ Proof.
   - lc_solve.
   - lc_solve.
   - lc_toplevel_inversion.
+(*
   - inversion IHPar1. constructor; auto.
   - inversion IHPar1. constructor; auto.
-  - inversion IHPar. constructor; auto.
+  - inversion IHPar. constructor; auto. *)
 Qed.
 
 Hint Resolve Par_lc1 Par_lc2 : lc.
@@ -114,11 +113,11 @@ Proof. intros W a a' R H. induction H; eauto.
           erewrite co_subst_co_tm_intro; eauto.
           replace W with (nil ++ W); auto. eapply subst_co_erased; eauto.
         - eapply erased_sub. eapply toplevel_erased1; eauto. auto.
-        - inversion IHPar1; eauto.
+(*        - inversion IHPar1; eauto.
         - inversion IHPar1; eauto.
         - inversion IHPar; eauto.
-        - econstructor. admit.
-Admitted.
+        - econstructor. admit. *)
+Qed.
 
 Lemma multipar_erased_tm_snd : forall W a a' R, multipar W a a' R ->
                                                erased_tm W a' R.
@@ -148,6 +147,7 @@ Lemma Par_sub: forall W a a' R1 R2, Par W a a' R1 -> SubRole R1 R2 ->
 Proof. intros W a a' R1 R2 H SR. generalize dependent R2.
        induction H; intros; simpl; eauto. econstructor.
        eapply erased_sub; eauto.
+       econstructor; eauto.
 Qed.
 
 Lemma multipar_sub : forall W a a' R1 R2, multipar W a a' R1 ->
@@ -195,7 +195,6 @@ Proof.
      rewrite tm_subst_tm_tm_open_tm_wrt_co_var; auto 1.
      rewrite tm_subst_tm_tm_open_tm_wrt_co_var; auto 1. eapply H0; eauto.
      eapply Par_lc2; eauto. eapply Par_lc1; eauto.
-   - econstructor; eauto.
    - econstructor; eauto.
    - econstructor; eauto.
 Qed.
@@ -256,14 +255,14 @@ Proof.
     apply Typing_context_fv in H.
     split_hyp. simpl in *.
     fsetdec.
-  - pose (P := IHPAR _ _ _ _ ltac:(auto) E). simpl in P. auto.
+(*  - pose (P := IHPAR _ _ _ _ ltac:(auto) E). simpl in P. auto.
   - econstructor; eauto 2. pose (P := IHPAR1 _ _ _ _ ltac:(auto) E).
     simpl in P. auto.
   - eapply Par_PushCombine; eauto 2. pose (P := IHPAR1 _ _ _ _ ltac:(auto) E).
     simpl in P. auto. pose (P := IHPAR2 _ _ _ _ ltac:(auto) E).
     simpl in P. auto.
   - econstructor; eauto. pose (P := IHPAR _ _ _ _ ltac:(auto) E).
-    simpl in P. auto.
+    simpl in P. auto. *)
 Qed.
 
 
@@ -296,14 +295,14 @@ Proof.
     apply Typing_context_fv in H.
     split_hyp. simpl in *.
     fsetdec.
-  - pose (P := IHPar _ _ _ _ ltac:(auto) H0). simpl in P. auto.
+(*  - pose (P := IHPar _ _ _ _ ltac:(auto) H0). simpl in P. auto.
   - econstructor; eauto 2. pose (P := IHPar1 _ _ _ _ ltac:(auto) H1).
     simpl in P. auto.
   - eapply Par_PushCombine; eauto 2. pose (P := IHPar1 _ _ _ _ ltac:(auto) H1).
     simpl in P. auto. pose (P := IHPar2 _ _ _ _ ltac:(auto) H1).
     simpl in P. auto.
   - econstructor; eauto. pose (P := IHPar _ _ _ _ ltac:(auto) H0).
-    simpl in P. auto.
+    simpl in P. auto. *)
 Qed.
 
 Lemma subst4 : forall b x, lc_co b ->
@@ -365,7 +364,7 @@ Hint Resolve erased_tm_open_tm_wrt_tm : erased.
 
 
 Lemma Par_Pi_exists: ∀ x W rho (A B A' B' : tm) R R',
-    x `notin` fv_tm_tm_tm B -> Par W A A' R
+    x `notin` fv_tm_tm_tm B -> Par W A A' R'
     → Par ([(x,R)] ++ W) (open_tm_wrt_tm B (a_Var_f x)) B' R'
     → Par W (a_Pi rho A R B) (a_Pi rho A' R (close_tm_wrt_tm x B')) R'.
 Proof.
@@ -382,8 +381,8 @@ Proof.
 Qed.
 
 Lemma Par_CPi_exists:  ∀ c W (A B a A' B' a' T T': tm) R R',
-       c `notin` fv_co_co_tm a -> Par W A A' R
-       → Par W B B' R -> Par W T T' R
+       c `notin` fv_co_co_tm a -> Par W A A' R'
+       → Par W B B' R' -> Par W T T' R'
          → Par W (open_tm_wrt_co a (g_Var_f c)) (a') R'
          → Par W (a_CPi (Eq A B T R) a) (a_CPi (Eq A' B' T' R) (close_tm_wrt_co c a')) R'.
 Proof.
@@ -456,7 +455,7 @@ Qed.
 
 Lemma multipar_Pi_exists: ∀ x W rho (A B A' B' : tm) R R',
        x `notin` fv_tm_tm_tm B ->
-       multipar W A A' R
+       multipar W A A' R'
        → multipar ([(x,R)] ++ W) (open_tm_wrt_tm B (a_Var_f x)) B' R'
        → multipar W (a_Pi rho A R B) (a_Pi rho A' R (close_tm_wrt_tm x B')) R'.
 Proof.
@@ -485,7 +484,7 @@ Qed.
 
 Lemma multipar_Pi_A_proj: ∀ W rho (A B A' B' : tm) R R',
     multipar W (a_Pi rho A R B) (a_Pi rho A' R B') R' ->
-    multipar W A A' R.
+    multipar W A A' R'.
 Proof.
   intros W rho A B A' B' R R' h1.
   dependent induction h1.
@@ -513,9 +512,9 @@ Qed.
 
 Lemma multipar_CPi_exists:  ∀ c W (A B a T A' B' a' T': tm) R R',
        c `notin` fv_co_co_tm a ->
-       multipar W A A' R →
-       multipar W B B' R ->
-       multipar W T T' R →
+       multipar W A A' R' →
+       multipar W B B' R' ->
+       multipar W T T' R' →
        multipar W (open_tm_wrt_co a (g_Var_f c)) a' R' →
        multipar W (a_CPi (Eq A B T R) a) (a_CPi (Eq A' B' T' R) (close_tm_wrt_co c a')) R'.
 Proof.
@@ -572,9 +571,9 @@ Qed.
 
 Lemma multipar_CPi_phi_proj:  ∀ W (A B a A' B' a' T T': tm) R R',
     multipar W (a_CPi (Eq A B T R) a) (a_CPi (Eq A' B' T' R) a') R' ->
-    multipar W A A' R 
-      /\ multipar W B B' R
-      /\ multipar W T T' R.
+    multipar W A A' R' 
+      /\ multipar W B B' R'
+      /\ multipar W T T' R'.
 Proof.
   intros W A B a A' B' a' T T' R R' H.
   dependent induction H; eauto.
@@ -662,8 +661,9 @@ Proof.
   eauto.
 Qed.
 
+(*
 Lemma multipar_Cast_exists : forall W a1 a2 R R', multipar W a1 a2 R ->
                multipar W (a_Conv a1 R' g_Triv) (a_Conv a2 R' g_Triv) R.
 Proof. intros. induction H. econstructor. econstructor. auto.
        econstructor. eapply Par_Cong; eauto. auto.
-Qed.
+Qed. *)
